cava/cava/Cava/Arrow/Instances/Prop.v
@@ -1,0 +1,193 @@
+From Coq Require Import Bool List ZArith Setoid Classes.Morphisms NaryFunctions VectorDef.
+Import ListNotations.
+Import VectorNotations.
+
+Require Import Cava.Arrow.Arrow.
+Require Import Cava.Arrow.Instances.Constructive.
+
+#[refine] Instance ConjPropKindCategory : Category Kind := {
+  morphism X Y := Prop;
+  compose _ _ _ f g := f /\ g;
+  id X := True;
+
+  morphism_equivalence x y f g := f <-> g;
+}.
+Proof.
+  - split. intros. inversion H. auto. intros. split; auto.
+  - split. intros. inversion H. auto. intros. split; auto.
+  - split. 
+    * intros. inversion H. inversion H1. auto.
+    * intros. inversion H. inversion H0. auto.
+Defined.
+
+#[refine] Instance ConjPropKindArrow : Arrow _ ConjPropKindCategory Unit Tuple := {
+  first _ _ _ p := p;
+  second _ _ _ p := p;
+
+  cancelr X := True;
+  cancell X := True;
+
+  uncancell _ := True;
+  uncancelr _ := True;
+
+  assoc _ _ _ := True;
+  unassoc _ _ _ := True;
+}.
+Proof.
+  - cbn. tauto.
+  - cbn. tauto.
+  - cbn. tauto.
+  - cbn. tauto.
+  - cbn. tauto.
+  - cbn. tauto.
+Defined.
+
+Instance TrueDrop : ArrowDrop ConjPropKindArrow := { drop _ := True }.
+Instance TrueCopy : ArrowCopy ConjPropKindArrow := { copy _ := True }.
+Instance TrueSwap : ArrowSwap ConjPropKindArrow := { swap _ _ := True }.
+
+Instance SubLoop : ArrowLoop ConjPropKindArrow := { loopl _ _ _ l := l; loopr _ _ _ l := l }.
+Instance FalseLoop : ArrowLoop ConjPropKindArrow := { loopl _ _ _ _ := False; loopr _ _ _ _ := False }.
+
+Instance NoDelays : Cava := {
+  cava_arrow := ConjPropKindArrow;
+  cava_arrow_loop := SubLoop;
+
+  constant b := True;
+  constant_bitvec n v := True;
+  not_gate := True;
+  and_gate := True;
+  nand_gate := True;
+  or_gate := True;
+  nor_gate := True;
+  xor_gate := True;
+  xnor_gate := True;
+  buf_gate := True;
+  xorcy := True;
+  muxcy := True;
+  unsigned_add _ _ _ := True;
+  lut _ _ := True;
+  index_vec n o := True;
+  slice_vec n x y o _ _ := True;
+  to_vec o := True;
+  append n o := True;
+  concat n m o := True;
+  split n m o H := True;
+
+  delay_gate _ := False;
+}.
+
+Instance NoLoops : Cava := {
+  cava_arrow := ConjPropKindArrow;
+  cava_arrow_loop := FalseLoop;
+
+  constant b := True;
+  constant_bitvec n v := True;
+  not_gate := True;
+  and_gate := True;
+  nand_gate := True;
+  or_gate := True;
+  nor_gate := True;
+  xor_gate := True;
+  xnor_gate := True;
+  buf_gate := True;
+  xorcy := True;
+  muxcy := True;
+  unsigned_add _ _ _ := True;
+  lut _ _ := True;
+  index_vec n o := True;
+  slice_vec n x y o _ _ := True;
+  to_vec o := True;
+  append n o := True;
+  concat n m o := True;
+  split n m o H := True;
+  delay_gate _ := True;
+}.
+
+(* Instance WfIndexing : Cava := {
+  cava_arrow := ConjPropKindArrow;
+  cava_arrow_loop := SubLoop;
+
+  constant b := True;
+  constant_bitvec n v := True;
+  not_gate := True;
+  and_gate := True;
+  nand_gate := True;
+  or_gate := True;
+  nor_gate := True;
+  xor_gate := True;
+  xnor_gate := True;
+  buf_gate := True;
+  xorcy := True;
+  muxcy := True;
+  unsigned_add _ _ _ := True;
+  lut _ _ := True;
+  slice_vec n x y o _ _ := True;
+  to_vec o := True;
+  append n o := True;
+  concat n m o := True;
+  split n m o H := True;
+  delay_gate _ := True;
+
+  index_vec n o := forall x, x < Nat.log2_up n; (* this is not right; x needs to be related to the actual values it receives *)
+}. *)
+
+Definition is_combinational {i o: Kind} (c: forall (cava: Cava), i ~[cava]~> o) := 
+  c NoLoops /\ c NoDelays.
+
+Definition mkCombinational {i o: Kind} (c: forall (cava: Cava), i ~[cava]~> o)
+  : c NoLoops -> c NoDelays -> is_combinational c.
+Proof.
+  intros.
+  unfold is_combinational.
+  tauto.
+Qed.
+
+Lemma is_combinational_first: forall x y z circuit,
+  is_combinational (toCava (@First x y z circuit)) =   
+  is_combinational (toCava circuit).
+Proof.
+  intros.
+  tauto.
+Qed.
+
+Lemma is_combinational_second: forall x y z circuit,
+  is_combinational (toCava (@Second x y z circuit)) =   
+  is_combinational (toCava circuit).
+Proof.
+  intros.
+  tauto.
+Qed.
+
+Lemma decompose_combinational (x y z : Kind) (f: structure x y) (g: structure y z):
+  is_combinational (toCava (Compose g f)) -> 
+  is_combinational (toCava g) /\ is_combinational (toCava f).
+Proof.
+  intros.
+  unfold is_combinational in *.
+  cbn in H.
+  tauto.
+Qed.
+
+Section example.
+  Definition ex_loopr {x y z: Kind} (cava: Cava) (c: x**z ~[cava]~> y**z): x ~[cava]~> y
+    := loopr c.
+  Definition ex_loopl {x y z: Kind} (cava: Cava) (c: z**x ~[cava]~> z**y): x ~[cava]~> y
+    := loopl c.
+
+  Lemma loopl_is_not_combinational : forall (x y z: Kind) (c: forall (cava: Cava), z**x ~[cava]~> z**y),
+    ~ is_combinational (fun cava => ex_loopl cava (c cava)).
+  Proof.
+    intros.
+    unfold is_combinational.
+    tauto.
+  Qed.
+
+  Lemma loopr_is_not_combinational : forall (x y z: Kind) (c: forall (cava: Cava), x**z ~[cava]~> y**z),
+    ~ is_combinational (fun cava => ex_loopr cava (c cava)).
+  Proof.
+    intros.
+    unfold is_combinational.
+    tauto.
+  Qed.
+End example.
